dafny/old/Readme.md
@@ -1,3 +1,0 @@
-# Old versions
-
-Some different ways to define the same mathematic functions that we are not using anymore considering some issues around using them to create some proofs.
